

Question 3:

a.) $L(B_0, B_1) = \prod [P(Y_i = 1)^{y_i}] \times [P(Y_i = 0)^{1-y_i}]$

\prod represents the product over all observations ($i = 1$ to 4)
; $P(Y_i = 1)$ is the probability of Y_i being 1.

$$\rightarrow P(Y_i = 1) = \frac{1}{1 + e^{-(B_0 + B_1 x_i)}}$$

Likelihood function

$$\rightarrow L(B_0, B_1) = \prod [P(Y_i = 1)^{y_i}] \times [P(Y_i = 0)^{1-y_i}]$$

b.) $\log_{B_1} \{ L(B_0) = \sum [y_i \times \log(P(Y_i = 1)) + (1 - y_i) \times \log(1 - P(Y_i = 1))] \}$

\sum represents the sum over all observations

a. Likelihood function:

$$L(B_0, B_1) = \left(\frac{1}{1 + e^{-(B_0 + B_1 x_4)}} \right) \times \left(\frac{1}{1 + e^{-(B_0 + B_1 x_3)}} \right) \times$$

$$\left(\frac{1}{1 + e^{-(B_0 + B_1 x_2)}} \right) \times \left(\frac{1}{1 + e^{-(B_0 + B_1 x_1)}} \right)$$

b. Likelihood functions:

$$\log_{B_1} \{ L(B_0) = \log \left(\left(\frac{1}{1 + e^{-(B_0 + B_1 x_4)}} \right) \times \left(\frac{1}{1 + e^{-(B_0 + B_1 x_3)}} \right) \right.$$

$$\left. \times \left(\frac{1}{1 + e^{-(B_0 + B_1 x_2)}} \right) \times \left(\frac{1}{1 + e^{-(B_0 + B_1 x_1)}} \right) \right)$$